\documentclass[12pt]{article}
\usepackage{amsmath}
\usepackage{amsfonts}
\usepackage{amssymb}
\usepackage{vmargin}
\usepackage[utf8]{inputenc}

% \displaystyle is sooo important
\newcommand{\D}{\displaystyle}

\begin{document}
\setmargins{2.5cm}
{0.1cm}
{16.5cm}
{23.42cm}
{10pt}
{1cm}
{0pt}
{2cm}

\title{Ayudant\'ia Matem\'aticas Avanzadas I N.5}
\date{7 de Abril 2022}
\author{Daniel S\'anchez}
\maketitle

\begin{enumerate}
      \item $\D \sum_{k = 50}^{100} 2(k+4)$
      \item $\D \sum_{k = 3}^{50} \ln \left(\frac{k}{k+1}\right)$
      \item $\D \sum_{k = 1}^{n} k(k+2)$
      \item $\D \sum_{k = 1}^{n} k(k+1)(k+2)$
      \item $\D \sum_{k = 3}^{n} \frac{2}{k^2+2k}$
      \item Calcular $\D \sum_{k=1}^{100} a_k$, donde $(a_k)_{k \in \mathbb{N}}$ es la sucesi\'on definida por:
            $$a_k=\left\{
                  \begin{array}{ll}
                        \D \frac{3-2^k}{4}     & \mbox{ si } 1 \leq k \leq 50 \\[3\jot]
                        \D \sqrt{k+2}-\sqrt{k} & \mbox{ si } k > 50
                  \end{array}
                  \right.$$
      \item \textbf{Bonus}, dado $0 < p < 1$, determine $w \in \mathbb{R}$ tal que:
            $$\D \sum_{k = 1}^{n} w(1-p)^{k-1} = 1$$
\end{enumerate}


\pagebreak
\title{\LARGE{\textbf{F\'ormulas}}}
\maketitle
\begin{enumerate}
      \item $\D \sum_{k = 1}^{n} 1 = n $
      \item $\D \sum_{k = 1}^{n} c = nc $ , \textit{donde} $c \in \mathbb{R}$
      \item $\D \sum_{k = 1}^{n} k = \frac{n(n+1)}{2} $
      \item $\D \sum_{k = 1}^{n} k^2 = \frac{n(n+1)(2n+1)}{6} $
      \item $\D \sum_{k = 1}^{n} k^3 = {\left(\frac{n(n+1)}{2}\right)}^2 $
      \item $\D \sum_{k = m-l}^{n-l} a_{k+l} = \sum_{k = m}^{n} a_k = \sum_{k = m+l}^{n+l} a_{k-l}$, \textit{con} $l \leq m < n$.
      \item $\D \sum_{k = 1}^{n} r^k = \frac{r(1-r^n)}{1-r} $, donde $r \in \mathbb{R}-\{1\}$
      \item $\D \sum_{k = m}^{n} (a_k-a_{k+1}) = a_m-a_{n+1}$, con $1\leq m \leq n$. \textit{(Propiedad Telesc\'opica)}
      \item $\D \sum_{k = m}^{n} a_k = \sum_{k = 1}^{n} a_k - \sum_{k = 1}^{m-1} a_k $, \textit{con} $1 \leq m < n$.
      \item $\D \sum_{k = 1}^{n} a_k = \sum_{k = 1}^{m} a_k + \sum_{k = m+1}^{n} a_k $, \textit{con} $1 \leq m < n$.
\end{enumerate}
\end{document}